theories/iris/logrel/fundamental.v
@@ -39,12 +39,12 @@ Section Fundamental.
     let fe := fe_of_context F in
     let ψ := InstrT [] [] in
     run_codegen (compile_instr me fe (INop ψ)) wl = inr ((), wl', es') ->
-    ⊢ has_type_semantic sr mr M F L [] (to_e_list es') ψ L.
+    ⊢ have_instruction_type_sem sr mr M F L [] (to_e_list es') ψ L.
   Proof.
     (* This is currently following the compat_copy lemma very closely *)
     intros me fe ψ Hcompile.
     inv_cg_emit Hcompile.
-    unfold has_type_semantic.
+    unfold have_instruction_type_sem.
     destruct ψ eqn:Hψ.
     inversion Hψ; subst l l0.
     iIntros (? ? ? ? ? ?) "Henv Hinst Hlf".
@@ -105,9 +105,9 @@ Section Fundamental.
   Lemma compat_unreachable M F L L' wl wl' ψ es' :
     let me := me_of_context M mr in
     let fe := fe_of_context F in
-    has_type_ok F L ψ L' ->
+    has_instruction_type_ok F L ψ L' ->
     run_codegen (compile_instr me fe (IUnreachable ψ)) wl = inr ((), wl', es') ->
-    ⊢ has_type_semantic sr mr M F L [] (to_e_list es') ψ L'.
+    ⊢ have_instruction_type_sem sr mr M F L [] (to_e_list es') ψ L'.
   Admitted.
 
   Lemma subst_repr_closed_nop ρ :
@@ -130,13 +130,13 @@ Section Fundamental.
     has_copyability F τ ExCopy ->
     let ψ := InstrT [τ] [τ; τ] in
     run_codegen (compile_instr me fe (ICopy ψ)) wl = inr ((), wl', es') ->
-    ⊢ has_type_semantic sr mr M F L [] (to_e_list es') ψ L.
+    ⊢ have_instruction_type_sem sr mr M F L [] (to_e_list es') ψ L.
   Proof.
     intros me fe Hmono Hcopy ψ Hcompile.
     unfold compile_instr in Hcompile.
     cbn in Hcompile.
     inv_cg_bind Hcompile ρ wl1 es_nil es1 Htype_rep Hcompile.
-    unfold has_type_semantic.
+    unfold have_instruction_type_sem.
     destruct ψ eqn:Hψ.
     inversion Hψ; subst l l0.
     iIntros (? ? ? ? ? ?) "Henv Hinst Hlh".
@@ -192,15 +192,15 @@ Section Fundamental.
     has_dropability F τ ExDrop ->
     let ψ := InstrT [τ] [] in
     run_codegen (compile_instr me fe (IDrop ψ)) wl = inr ((), wl', es') ->
-    ⊢ has_type_semantic sr mr M F L [] (to_e_list es') ψ L.
+    ⊢ have_instruction_type_sem sr mr M F L [] (to_e_list es') ψ L.
   Admitted.
 
-  Lemma compat_num M F L wl wl' ψ eₙ es' :
+  Lemma compat_num M F L wl wl' ψ e es' :
     let me := me_of_context M mr in
     let fe := fe_of_context F in
-    num_instr_has_type eₙ ψ ->
-    run_codegen (compile_instr me fe (INum ψ eₙ)) wl = inr ((), wl', es') ->
-    ⊢ has_type_semantic sr mr M F L [] (to_e_list es') ψ L.
+    has_instruction_type_num e ψ ->
+    run_codegen (compile_instr me fe (INum ψ e)) wl = inr ((), wl', es') ->
+    ⊢ have_instruction_type_sem sr mr M F L [] (to_e_list es') ψ L.
   Admitted.
 
   Lemma compat_num_const M F L wl wl' n ν κ es' :
@@ -209,7 +209,7 @@ Section Fundamental.
     has_kind F (NumT κ ν) κ ->
     let ψ := InstrT [] [NumT κ ν] in
     run_codegen (compile_instr me fe (INumConst ψ n)) wl = inr ((), wl', es') ->
-    ⊢ has_type_semantic sr mr M F L [] (to_e_list es') ψ L.
+    ⊢ have_instruction_type_sem sr mr M F L [] (to_e_list es') ψ L.
   Admitted.
 
   Lemma compat_block M F L wl wl' ξ τs1 τs2 es es' :
@@ -218,13 +218,13 @@ Section Fundamental.
     let L' := update_locals ξ L in
     let F' := set fc_labels (cons (τs2, L')) F in
     let ψ := InstrT τs1 τs2 in
-    instrs_have_type M F' L es ψ L' ->
+    have_instruction_type M F' L es ψ L' ->
     (forall wl wl' es',
         let fe' := fe_of_context F' in
         run_codegen (compile_instrs me fe' es) wl = inr ((), wl', es') ->
-        ⊢ has_type_semantic sr mr M F' L wl' (to_e_list es') ψ L') ->
+        ⊢ have_instruction_type_sem sr mr M F' L wl' (to_e_list es') ψ L') ->
     run_codegen (compile_instr me fe (IBlock ψ ξ es)) wl = inr ((), wl', es') ->
-    ⊢ has_type_semantic sr mr M F L [] (to_e_list es') ψ L'.
+    ⊢ have_instruction_type_sem sr mr M F L [] (to_e_list es') ψ L'.
   Admitted.
 
   Lemma compat_loop M F L wl wl' es es' τs1 τs2 :
@@ -232,29 +232,29 @@ Section Fundamental.
     let fe := fe_of_context F in
     let F' := set fc_labels (cons (τs1, L)) F in
     let ψ := InstrT τs1 τs2 in
-    instrs_have_type M F' L es ψ L ->
+    have_instruction_type M F' L es ψ L ->
     (forall wl wl' es',
         let fe' := fe_of_context F' in
         run_codegen (compile_instrs me fe' es) wl = inr ((), wl', es') ->
-        ⊢ has_type_semantic sr mr M F' L wl' (to_e_list es') ψ L) ->
+        ⊢ have_instruction_type_sem sr mr M F' L wl' (to_e_list es') ψ L) ->
     run_codegen (compile_instr me fe (ILoop ψ es)) wl = inr ((), wl', es') ->
-    ⊢ has_type_semantic sr mr M F L [] (to_e_list es') ψ L.
+    ⊢ have_instruction_type_sem sr mr M F L [] (to_e_list es') ψ L.
   Admitted.
 
   Lemma compat_ite M F L wl wl' es1 es2 es' ξ ψ :
     let me := me_of_context M mr in
     let fe := fe_of_context F in
     let L' := update_locals ξ L in
-    instrs_have_type M F L es1 ψ L' ->
-    instrs_have_type M F L es2 ψ L' ->
+    have_instruction_type M F L es1 ψ L' ->
+    have_instruction_type M F L es2 ψ L' ->
     (forall wl wl' es',
         run_codegen (compile_instrs me fe es1) wl = inr ((), wl', es') ->
-        ⊢ has_type_semantic sr mr M F L wl' (to_e_list es') ψ L') ->
+        ⊢ have_instruction_type_sem sr mr M F L wl' (to_e_list es') ψ L') ->
     (forall wl wl' es',
         run_codegen (compile_instrs me fe es2) wl = inr ((), wl', es') ->
-        ⊢ has_type_semantic sr mr M F L wl' (to_e_list es') ψ L') ->
+        ⊢ have_instruction_type_sem sr mr M F L wl' (to_e_list es') ψ L') ->
     run_codegen (compile_instr me fe (IIte ψ ξ es1 es2)) wl = inr ((), wl', es') ->
-    ⊢ has_type_semantic sr mr M F L [] (to_e_list es') ψ L'.
+    ⊢ have_instruction_type_sem sr mr M F L [] (to_e_list es') ψ L'.
   Admitted.
 
   Lemma compat_br M F L wl wl' es' n τs1 τs τs2 ξ :
@@ -265,7 +265,7 @@ Section Fundamental.
     let ψ := InstrT (τs1 ++ τs) τs2 in
     let L' := update_locals ξ L in
     run_codegen (compile_instr me fe (IBr ψ n)) wl = inr ((), wl', es') ->
-    ⊢ has_type_semantic sr mr M F L [] (to_e_list es') ψ L'.
+    ⊢ have_instruction_type_sem sr mr M F L [] (to_e_list es') ψ L'.
   Admitted.
 
   Lemma compat_br_if M F L wl wl' es' n τs :
@@ -275,7 +275,7 @@ Section Fundamental.
     let τ := NumT (VALTYPE (PrimR I32R) ImCopy ImDrop) (IntT I32T) in
     let ψ := InstrT (τs ++ [τ]) τs in
     run_codegen (compile_instr me fe (IBrIf ψ n)) wl = inr ((), wl', es') ->
-    ⊢ has_type_semantic sr mr M F L [] (to_e_list es') ψ L.
+    ⊢ have_instruction_type_sem sr mr M F L [] (to_e_list es') ψ L.
   Admitted.
 
   Lemma compat_br_table M F L L' wl wl' es' n ns τs τs1 τs2 :
@@ -286,7 +286,7 @@ Section Fundamental.
     let τ := NumT (VALTYPE (PrimR I32R) ImCopy ImDrop) (IntT I32T) in
     let ψ := InstrT (τs1 ++ τs ++ [τ]) τs2 in
     run_codegen (compile_instr me fe (IBrTable ψ ns n)) wl = inr ((), wl', es') ->
-    ⊢ has_type_semantic sr mr M F L [] (to_e_list es') ψ L'.
+    ⊢ have_instruction_type_sem sr mr M F L [] (to_e_list es') ψ L'.
   Admitted.
 
   Lemma compat_return M F L L' wl wl' es' τs τs1 τs2 :
@@ -296,7 +296,7 @@ Section Fundamental.
     Forall (fun τ => has_dropability F τ ImDrop) τs1 ->
     let ψ := InstrT (τs1 ++ τs) τs2 in
     run_codegen (compile_instr me fe (IReturn ψ)) wl = inr ((), wl', es') ->
-    ⊢ has_type_semantic sr mr M F L [] (to_e_list es') ψ L'.
+    ⊢ have_instruction_type_sem sr mr M F L [] (to_e_list es') ψ L'.
   Admitted.
 
   Lemma compat_local_get M F L wl wl' es' n τ ρ :
@@ -308,7 +308,7 @@ Section Fundamental.
     let L' := <[n := τ']> L in
     let ψ := InstrT [] [τ] in
     run_codegen (compile_instr me fe (ILocalGet ψ n)) wl = inr ((), wl', es') ->
-    ⊢ has_type_semantic sr mr M F L [] (to_e_list es') ψ L'.
+    ⊢ have_instruction_type_sem sr mr M F L [] (to_e_list es') ψ L'.
   Admitted.
 
   Lemma compat_local_get_copy M F L wl wl' es' n τ :
@@ -318,7 +318,7 @@ Section Fundamental.
     has_copyability F τ ImCopy ->
     let ψ := InstrT [] [τ] in
     run_codegen (compile_instr me fe (ILocalGet ψ n)) wl = inr ((), wl', es') ->
-    ⊢ has_type_semantic sr mr M F L [] (to_e_list es') ψ L.
+    ⊢ have_instruction_type_sem sr mr M F L [] (to_e_list es') ψ L.
   Admitted.
 
   Lemma compat_local_set M F L wl wl' es' n τ τ' ρ ρ' :
@@ -332,7 +332,7 @@ Section Fundamental.
     let L' := <[n := τ']> L in
     let ψ := InstrT [τ'] [] in
     run_codegen (compile_instr me fe (ILocalSet ψ n)) wl = inr ((), wl', es') ->
-    ⊢ has_type_semantic sr mr M F L [] (to_e_list es') ψ L'.
+    ⊢ have_instruction_type_sem sr mr M F L [] (to_e_list es') ψ L'.
   Admitted.
 
   Lemma compat_global_get M F L wl wl' es' n m τ :
@@ -342,7 +342,7 @@ Section Fundamental.
     has_copyability F τ ImCopy ->
     let ψ := InstrT [] [τ] in
     run_codegen (compile_instr me fe (IGlobalGet ψ n)) wl = inr ((), wl', es') ->
-    ⊢ has_type_semantic sr mr M F L [] (to_e_list es') ψ L.
+    ⊢ have_instruction_type_sem sr mr M F L [] (to_e_list es') ψ L.
   Admitted.
 
   Lemma compat_global_set M F L wl wl' es' n τ :
@@ -352,7 +352,7 @@ Section Fundamental.
     has_dropability F τ ImDrop ->
     let ψ := InstrT [τ] [] in
     run_codegen (compile_instr me fe (IGlobalSet ψ n)) wl = inr ((), wl', es') ->
-    ⊢ has_type_semantic sr mr M F L [] (to_e_list es') ψ L.
+    ⊢ have_instruction_type_sem sr mr M F L [] (to_e_list es') ψ L.
   Admitted.
 
   Lemma compat_global_swap M F L wl wl' es' n τ :
@@ -361,7 +361,7 @@ Section Fundamental.
     mc_globals M !! n = Some (Mut, τ) ->
     let ψ := InstrT [τ] [τ] in
     run_codegen (compile_instr me fe (IGlobalSwap ψ n)) wl = inr ((), wl', es') ->
-    ⊢ has_type_semantic sr mr M F L [] (to_e_list es') ψ L.
+    ⊢ have_instruction_type_sem sr mr M F L [] (to_e_list es') ψ L.
   Admitted.
 
   Lemma compat_coderef M F L wl wl' es' i ϕ :
@@ -371,16 +371,16 @@ Section Fundamental.
     let τ := CodeRefT (VALTYPE (PrimR I32R) ImCopy ImDrop) ϕ in
     let ψ := InstrT [] [τ] in
     run_codegen (compile_instr me fe (ICodeRef ψ i)) wl = inr ((), wl', es') ->
-    ⊢ has_type_semantic sr mr M F L [] (to_e_list es') ψ L.
+    ⊢ have_instruction_type_sem sr mr M F L [] (to_e_list es') ψ L.
   Admitted.
 
   Lemma compat_inst M F L wl wl' es' ix ϕ ϕ' κ :
     let me := me_of_context M mr in
     let fe := fe_of_context F in
-    inst_function_type F ix ϕ ϕ' ->
+    function_type_inst F ix ϕ ϕ' ->
     let ψ := InstrT [CodeRefT κ ϕ] [CodeRefT κ ϕ'] in
     run_codegen (compile_instr me fe (IInst ψ ix)) wl = inr ((), wl', es') ->
-    ⊢ has_type_semantic sr mr M F L [] (to_e_list es') ψ L.
+    ⊢ have_instruction_type_sem sr mr M F L [] (to_e_list es') ψ L.
   Admitted.
 
   Lemma compat_call M F L wl wl' es' i ixs ϕ τs1 τs2 :
@@ -388,9 +388,9 @@ Section Fundamental.
     let fe := fe_of_context F in
     mc_functions M !! i = Some ϕ ->
     let ψ := InstrT τs1 τs2 in
-    list_inst_function_type F ixs ϕ (MonoFunT ψ) ->
+    function_type_insts F ixs ϕ (MonoFunT ψ) ->
     run_codegen (compile_instr me fe (ICall ψ i ixs)) wl = inr ((), wl', es') ->
-    ⊢ has_type_semantic sr mr M F L [] (to_e_list es') ψ L.
+    ⊢ have_instruction_type_sem sr mr M F L [] (to_e_list es') ψ L.
   Admitted.
 
   Lemma compat_call_indirect M F L wl wl' es' τs1 τs2 κ :
@@ -398,7 +398,7 @@ Section Fundamental.
     let fe := fe_of_context F in
     let ψ := InstrT (τs1 ++ [CodeRefT κ (MonoFunT (InstrT τs1 τs2))]) τs2 in
     run_codegen (compile_instr me fe (ICallIndirect ψ)) wl = inr ((), wl', es') ->
-    ⊢ has_type_semantic sr mr M F L [] (to_e_list es') ψ L.
+    ⊢ have_instruction_type_sem sr mr M F L [] (to_e_list es') ψ L.
   Admitted.
 
   Lemma compat_inject M F L wl wl' es' i τs τ κ :
@@ -407,17 +407,17 @@ Section Fundamental.
     τs !! i = Some τ ->
     let ψ := InstrT [τ] [SumT κ τs] in
     run_codegen (compile_instr me fe (IInject ψ i)) wl = inr ((), wl', es') ->
-    ⊢ has_type_semantic sr mr M F L [] (to_e_list es') ψ L.
+    ⊢ have_instruction_type_sem sr mr M F L [] (to_e_list es') ψ L.
   Admitted.
 
   Lemma compat_case M F L wl wl' es' ξ ess τ' τs κ :
     let me := me_of_context M mr in
     let fe := fe_of_context F in
     let L' := update_locals ξ L in
-    Forall2 (fun τ es => instrs_have_type M F L es (InstrT [τ] [τ']) L') τs ess ->
+    Forall2 (fun τ es => have_instruction_type M F L es (InstrT [τ] [τ']) L') τs ess ->
     let ψ := InstrT [SumT κ τs] [τ'] in
     run_codegen (compile_instr me fe (ICase ψ ξ ess)) wl = inr ((), wl', es') ->
-    ⊢ has_type_semantic sr mr M F L [] (to_e_list es') ψ L'.
+    ⊢ have_instruction_type_sem sr mr M F L [] (to_e_list es') ψ L'.
   Admitted.
 
   Lemma compat_group M F L wl wl' es' τs ρs χ δ :
@@ -427,7 +427,7 @@ Section Fundamental.
     let τ := ProdT (VALTYPE (ProdR ρs) χ δ) τs in
     let ψ := InstrT τs [τ] in
     run_codegen (compile_instr me fe (IGroup ψ)) wl = inr ((), wl', es') ->
-    ⊢ has_type_semantic sr mr M F L [] (to_e_list es') ψ L.
+    ⊢ have_instruction_type_sem sr mr M F L [] (to_e_list es') ψ L.
   Admitted.
 
   Lemma compat_ungroup M F L wl wl' es' τs κ :
@@ -436,7 +436,7 @@ Section Fundamental.
     let τ := ProdT κ τs in
     let ψ := InstrT [τ] τs in
     run_codegen (compile_instr me fe (IUngroup ψ)) wl = inr ((), wl', es') ->
-    ⊢ has_type_semantic sr mr M F L [] (to_e_list es') ψ L.
+    ⊢ have_instruction_type_sem sr mr M F L [] (to_e_list es') ψ L.
   Admitted.
 
   Lemma compat_fold M F L wl wl' es' τ κ :
@@ -446,7 +446,7 @@ Section Fundamental.
     let τ0 := subst_type VarM VarR VarS (unscoped.scons (RecT κ τ) VarT) τ in
     let ψ := InstrT [τ0] [RecT κ τ] in
     run_codegen (compile_instr me fe (IFold ψ)) wl = inr ((), wl', es') ->
-    ⊢ has_type_semantic sr mr M F L [] (to_e_list es') ψ L.
+    ⊢ have_instruction_type_sem sr mr M F L [] (to_e_list es') ψ L.
   Admitted.
 
   Lemma compat_unfold M F L wl wl' es' τ κ :
@@ -455,16 +455,16 @@ Section Fundamental.
     let τ0 := subst_type VarM VarR VarS (unscoped.scons (RecT κ τ) VarT) τ in
     let ψ := InstrT [RecT κ τ] [τ0] in
     run_codegen (compile_instr me fe (IUnfold ψ)) wl = inr ((), wl', es') ->
-    ⊢ has_type_semantic sr mr M F L [] (to_e_list es') ψ L.
+    ⊢ have_instruction_type_sem sr mr M F L [] (to_e_list es') ψ L.
   Admitted.
 
   Lemma compat_pack M F L wl wl' es' τ τ' :
     let me := me_of_context M mr in
     let fe := fe_of_context F in
-    pack_existential_type F τ τ' ->
+    packed_existential_type F τ τ' ->
     let ψ := InstrT [τ] [τ'] in
     run_codegen (compile_instr me fe (IPack ψ)) wl = inr ((), wl', es') ->
-    ⊢ has_type_semantic sr mr M F L [] (to_e_list es') ψ L.
+    ⊢ have_instruction_type_sem sr mr M F L [] (to_e_list es') ψ L.
   Admitted.
 
   Lemma compat_unpack_mem M F L wl wl' es es' ξ τ τs1 τs2 κ :
@@ -475,16 +475,17 @@ Section Fundamental.
     let L' := update_locals ξ L in
     let weak_t := map (subst_type (up_memory VarM) VarR VarS VarT) in
     let weak_e := map (subst_instruction (up_memory VarM) VarR VarS VarT) in
-    instrs_have_type M F' (weak_t L) (weak_e es) (InstrT (weak_t τs1 ++ [τ]) (weak_t τs2)) (weak_t L') ->
+    have_instruction_type
+      M F' (weak_t L) (weak_e es) (InstrT (weak_t τs1 ++ [τ]) (weak_t τs2)) (weak_t L') ->
     let ψ := InstrT (τs1 ++ [ExistsMemT κ τ]) τs2 in
     (forall wl wl' es',
         let fe' := fe_of_context F' in
         run_codegen (compile_instrs me fe' (weak_e es)) wl = inr ((), wl', es') ->
-        ⊢ has_type_semantic sr mr M F' (weak_t L) wl'
+        ⊢ have_instruction_type_sem sr mr M F' (weak_t L) wl'
           (to_e_list es')
           (InstrT (weak_t τs1 ++ [τ]) (weak_t τs2)) (weak_t L')) ->
     run_codegen (compile_instr me fe (IUnpack ψ ξ es)) wl = inr ((), wl', es') ->
-    ⊢ has_type_semantic sr mr M F L [] (to_e_list es') ψ L'.
+    ⊢ have_instruction_type_sem sr mr M F L [] (to_e_list es') ψ L'.
   Admitted.
 
   Lemma compat_unpack_rep M F L wl wl' es es' ξ τ τs1 τs2 κ :
@@ -495,16 +496,17 @@ Section Fundamental.
     let L' := update_locals ξ L in
     let weak_t := map (subst_type VarM (up_representation VarR) VarS VarT) in
     let weak_e := map (subst_instruction VarM (up_representation VarR) VarS VarT) in
-    instrs_have_type M F' (weak_t L) (weak_e es) (InstrT (weak_t τs1 ++ [τ]) (weak_t τs2)) (weak_t L') ->
+    have_instruction_type
+      M F' (weak_t L) (weak_e es) (InstrT (weak_t τs1 ++ [τ]) (weak_t τs2)) (weak_t L') ->
     let ψ := InstrT (τs1 ++ [ExistsRepT κ τ]) τs2 in
     (forall wl wl' es',
         let fe' := fe_of_context F' in
         run_codegen (compile_instrs me fe' (weak_e es)) wl = inr ((), wl', es') ->
-        ⊢ has_type_semantic sr mr M F' (weak_t L) wl'
+        ⊢ have_instruction_type_sem sr mr M F' (weak_t L) wl'
           (to_e_list es')
           (InstrT (weak_t τs1 ++ [τ]) (weak_t τs2)) (weak_t L')) ->
     run_codegen (compile_instr me fe (IUnpack ψ ξ es)) wl = inr ((), wl', es') ->
-    ⊢ has_type_semantic sr mr M F L [] (to_e_list es') ψ L'.
+    ⊢ have_instruction_type_sem sr mr M F L [] (to_e_list es') ψ L'.
   Admitted.
 
   Lemma compat_unpack_size M F L wl wl' es es' ξ τ τs1 τs2 κ :
@@ -515,16 +517,17 @@ Section Fundamental.
     let L' := update_locals ξ L in
     let weak_t := map (subst_type VarM VarR (up_size VarS) VarT) in
     let weak_e := map (subst_instruction VarM VarR (up_size VarS) VarT) in
-    instrs_have_type M F' (weak_t L) (weak_e es) (InstrT (weak_t τs1 ++ [τ]) (weak_t τs2)) (weak_t L') ->
+    have_instruction_type
+      M F' (weak_t L) (weak_e es) (InstrT (weak_t τs1 ++ [τ]) (weak_t τs2)) (weak_t L') ->
     let ψ := InstrT (τs1 ++ [ExistsRepT κ τ]) τs2 in
     (forall wl wl' es',
         let fe' := fe_of_context F' in
         run_codegen (compile_instrs me fe' (weak_e es)) wl = inr ((), wl', es') ->
-        ⊢ has_type_semantic sr mr M F' (weak_t L) wl'
+        ⊢ have_instruction_type_sem sr mr M F' (weak_t L) wl'
           (to_e_list es')
           (InstrT (weak_t τs1 ++ [τ]) (weak_t τs2)) (weak_t L')) ->
     run_codegen (compile_instr me fe (IUnpack ψ ξ es)) wl = inr ((), wl', es') ->
-    ⊢ has_type_semantic sr mr M F L [] (to_e_list es') ψ L'.
+    ⊢ have_instruction_type_sem sr mr M F L [] (to_e_list es') ψ L'.
   Admitted.
 
   Lemma compat_unpack_type M F L wl wl' es es' ξ τ τs1 τs2 κ κ0 :
@@ -535,16 +538,17 @@ Section Fundamental.
     let L' := update_locals ξ L in
     let weak_t := map (subst_type VarM VarR VarS (up_type VarT)) in
     let weak_e := map (subst_instruction VarM VarR VarS (up_type VarT)) in
-    instrs_have_type M F' (weak_t L) (weak_e es) (InstrT (weak_t τs1 ++ [τ]) (weak_t τs2)) (weak_t L') ->
+    have_instruction_type
+      M F' (weak_t L) (weak_e es) (InstrT (weak_t τs1 ++ [τ]) (weak_t τs2)) (weak_t L') ->
     let ψ := InstrT (τs1 ++ [ExistsTypeT κ κ0 τ]) τs2 in
     (forall wl wl' es',
         let fe' := fe_of_context F' in
         run_codegen (compile_instrs me fe' (weak_e es)) wl = inr ((), wl', es') ->
-        ⊢ has_type_semantic sr mr M F' (weak_t L) wl'
+        ⊢ have_instruction_type_sem sr mr M F' (weak_t L) wl'
           (to_e_list es')
           (InstrT (weak_t τs1 ++ [τ]) (weak_t τs2)) (weak_t L')) ->
     run_codegen (compile_instr me fe (IUnpack ψ ξ es)) wl = inr ((), wl', es') ->
-    ⊢ has_type_semantic sr mr M F L [] (to_e_list es') ψ L'.
+    ⊢ have_instruction_type_sem sr mr M F L [] (to_e_list es') ψ L'.
   Admitted.
 
   Lemma compat_wrap M F L wl wl' es' τ0 ρ0 ρ ιs0 ιs χ δ :
@@ -557,7 +561,7 @@ Section Fundamental.
     let τ := RepT (VALTYPE ρ χ δ) ρ τ0 in
     let ψ := InstrT [τ0] [τ] in
     run_codegen (compile_instr me fe (IWrap ψ)) wl = inr ((), wl', es') ->
-    ⊢ has_type_semantic sr mr M F L [] (to_e_list es') ψ L.
+    ⊢ have_instruction_type_sem sr mr M F L [] (to_e_list es') ψ L.
   Admitted.
 
   Lemma compat_unwrap M F L wl wl' es' τ0 ρ0 ρ ιs0 ιs χ δ :
@@ -570,7 +574,7 @@ Section Fundamental.
     let τ := RepT (VALTYPE ρ χ δ) ρ τ0 in
     let ψ := InstrT [τ] [τ0] in
     run_codegen (compile_instr me fe (IUnwrap ψ)) wl = inr ((), wl', es') ->
-    ⊢ has_type_semantic sr mr M F L [] (to_e_list es') ψ L.
+    ⊢ have_instruction_type_sem sr mr M F L [] (to_e_list es') ψ L.
   Admitted.
 
   Lemma compat_ref_new M F L wl wl' es' μ τ τ' κ :
@@ -582,7 +586,7 @@ Section Fundamental.
     has_kind F τ κ ->
     let ψ := InstrT [τ] [τ_ref] in
     run_codegen (compile_instr me fe (IRefNew ψ)) wl = inr ((), wl', es') ->
-    ⊢ has_type_semantic sr mr M F L [] (to_e_list es') ψ L.
+    ⊢ have_instruction_type_sem sr mr M F L [] (to_e_list es') ψ L.
   Admitted.
 
   Lemma compat_ref_load M F L wl wl' es' μ π τ τ_val pr ρ δ κ :
@@ -597,7 +601,7 @@ Section Fundamental.
     has_kind F τ_ref κ ->
     let ψ := InstrT [τ_ref] [τ_ref; τ_val] in
     run_codegen (compile_instr me fe (IRefLoad ψ π)) wl = inr ((), wl', es') ->
-    ⊢ has_type_semantic sr mr M F L [] (to_e_list es') ψ L.
+    ⊢ have_instruction_type_sem sr mr M F L [] (to_e_list es') ψ L.
   Admitted.
 
   Lemma compat_ref_store M F L wl wl' es' μ π τ τ_val pr κ :
@@ -610,7 +614,7 @@ Section Fundamental.
     let τ_ref := RefT κ μ τ in
     let ψ := InstrT [τ_ref; τ_val] [τ] in
     run_codegen (compile_instr me fe (IRefStore ψ π)) wl = inr ((), wl', es') ->
-    ⊢ has_type_semantic sr mr M F L [] (to_e_list es') ψ L.
+    ⊢ have_instruction_type_sem sr mr M F L [] (to_e_list es') ψ L.
   Admitted.
 
   Lemma compat_ref_mm_store M F L wl wl' es' π τ τ_val τ_val' pr κ κ' σ σ' δ :
@@ -628,7 +632,7 @@ Section Fundamental.
     has_kind F τ_ref' κ' ->
     let ψ := InstrT [τ_ref; τ_val] [τ_ref'] in
     run_codegen (compile_instr me fe (IRefStore ψ π)) wl = inr ((), wl', es') ->
-    ⊢ has_type_semantic sr mr M F L [] (to_e_list es') ψ L.
+    ⊢ have_instruction_type_sem sr mr M F L [] (to_e_list es') ψ L.
   Admitted.
 
   Lemma compat_ref_swap M F L wl wl' es' π τ τ_val pr κ μ :
@@ -640,7 +644,7 @@ Section Fundamental.
     let τ_ref := RefT κ μ τ in
     let ψ := InstrT [τ_ref; τ_val] [τ_ref; τ_val] in
     run_codegen (compile_instr me fe (IRefSwap ψ π)) wl = inr ((), wl', es') ->
-    ⊢ has_type_semantic sr mr M F L [] (to_e_list es') ψ L.
+    ⊢ have_instruction_type_sem sr mr M F L [] (to_e_list es') ψ L.
   Admitted.
 
   Lemma compat_ref_mm_swap M F L wl wl' es' π τ τ_val τ_val' τ__π κ κ' pr :
@@ -657,49 +661,49 @@ Section Fundamental.
     has_kind F τ_ref' κ' ->
     let ψ := InstrT [τ_ref; τ_val] [τ_ref'; τ__π] in
     run_codegen (compile_instr me fe (IRefSwap ψ π)) wl = inr ((), wl', es') ->
-    ⊢ has_type_semantic sr mr M F L [] (to_e_list es') ψ L.
+    ⊢ have_instruction_type_sem sr mr M F L [] (to_e_list es') ψ L.
   Admitted.
 
   Lemma compat_nil M F L wl wl' es' :
     let me := me_of_context M mr in
     let fe := fe_of_context F in
     run_codegen (compile_instrs me fe []) es' = inr ((), wl, wl') ->
-    ⊢ has_type_semantic sr mr M F L wl (to_e_list wl') (InstrT [] []) L.
+    ⊢ have_instruction_type_sem sr mr M F L wl (to_e_list wl') (InstrT [] []) L.
   Admitted.
 
   Lemma compat_cons M F L1 L2 L3 wl wl' es' e es τs1 τs2 τs3 :
     let me := me_of_context M mr in
     let fe := fe_of_context F in
-    instr_has_type M F L1 e (InstrT τs1 τs2) L2 ->
-    instrs_have_type M F L2 es (InstrT τs2 τs3) L3 ->
+    has_instruction_type M F L1 e (InstrT τs1 τs2) L2 ->
+    have_instruction_type M F L2 es (InstrT τs2 τs3) L3 ->
     (forall es' wl wl',
         run_codegen (compile_instr me fe e) wl = inr ((), wl', es') ->
-        ⊢ has_type_semantic sr mr M F L1 [] (to_e_list es') (InstrT τs1 τs2) L2) ->
+        ⊢ have_instruction_type_sem sr mr M F L1 [] (to_e_list es') (InstrT τs1 τs2) L2) ->
     (forall wl wl' es',
         run_codegen (compile_instrs me fe es) wl = inr ((), wl', es') ->
-        ⊢ has_type_semantic sr mr M F L2 wl' (to_e_list es') (InstrT τs2 τs3) L3) ->
+        ⊢ have_instruction_type_sem sr mr M F L2 wl' (to_e_list es') (InstrT τs2 τs3) L3) ->
     run_codegen (compile_instrs me fe (e :: es)) es' = inr ((), wl, wl') ->
-    ⊢ has_type_semantic sr mr M F L1 wl (to_e_list wl') (InstrT τs1 τs3) L3.
+    ⊢ have_instruction_type_sem sr mr M F L1 wl (to_e_list wl') (InstrT τs1 τs3) L3.
   Admitted.
 
   Theorem fundamental_theorem M F L L' wl wl' es es' tf :
-    instrs_have_type M F L es tf L' ->
+    have_instruction_type M F L es tf L' ->
     let me := me_of_context M mr in
     let fe := fe_of_context F in
     run_codegen (compile_instrs me fe es) wl = inr (tt, wl', es') ->
-    ⊢ has_type_semantic sr mr M F L wl' (to_e_list es') tf L'.
+    ⊢ have_instruction_type_sem sr mr M F L wl' (to_e_list es') tf L'.
   Proof.
     intros Htype.
     generalize dependent es'.
     generalize dependent wl'.
     generalize dependent wl.
-    induction Htype using instrs_have_type_mind with
+    induction Htype using have_instruction_type_mind with
       (P := fun M F L e ψ L' _ =>
               forall es' wl wl',
                 let me := me_of_context M mr in
                 let fe := fe_of_context F in
                 run_codegen (compile_instr me fe e) wl = inr (tt, wl', es') ->
-                ⊢ has_type_semantic sr mr M F L [] (to_e_list es') ψ L');
+                ⊢ have_instruction_type_sem sr mr M F L [] (to_e_list es') ψ L');
       intros es' wl wl' me fe Hcomp.
     - eapply compat_nop; eassumption.
     - eapply compat_unreachable; eassumption.
